Updated Algorithm to the Proposal one.

Rocq/src/Algo.v
@@ -5,8 +5,8 @@ From Stdlib Require Import Logic.FunctionalExtensionality.
 
 From Verilog Require Import Expr.
 From Verilog Require Import ExprPath.
-From Verilog Require Import TypedExpr.
-From Verilog Require Import TypedExprPath.
+From Verilog Require Import TaggedExpr.
+From Verilog Require Import TaggedExprPath.
 From Verilog Require Import TypeSystem.
 From Verilog Require Import Spec.
 From Verilog Require Import Utils.
@@ -17,96 +17,113 @@ Import ListNotations.
 Import Path.
 Import Expr.
 Import ExprPath.
-Import TypedExpr.
-Import TypedExprPath.
+Import TaggedExpr.
+Import TaggedExprPath.
 Import TypeSystem.
-Import Spec.
 Import Utils.
 Import Learn.
 
 Module Algo.
-  Fixpoint down s e :=
+  Fixpoint determine e :=
     match e with
-    | TAtom _ op => TAtom s op
-    | TBinOp _ tLhs tRhs => TBinOp s (down s tLhs) (down s tRhs)
-    | TUnOp _ tArg => TUnOp s (down s tArg)
-    | TCast _ tArg => TCast s (down (size tArg) tArg)
-    | TComp _ tLhs tRhs =>
-        let sArg := max (size tLhs) (size tRhs) in
-        TComp s (down sArg tLhs) (down sArg tRhs)
-    | TLogic _ tLhs tRhs => TLogic s (down (size tLhs) tLhs) (down (size tRhs) tRhs)
-    | TReduction _ tArg => TReduction s (down (size tArg) tArg)
-    | TShift _ tLhs tRhs => TShift s (down s tLhs) (down (size tRhs) tRhs)
-    | TAssign _ lval tArg =>
-        let sArg := max lval (size tArg) in
-        TAssign s lval (down sArg tArg)
-    | TCond _ tArg tLhs tRhs => TCond s (down (size tArg) tArg) (down s tLhs) (down s tRhs)
-    | TConcat _ tArgs =>
-        TConcat s (map (fun tE => down (size tE) tE) tArgs)
-    | TRepl _ n tArg => TRepl s n (down (size tArg) tArg)
-    end
-  .
-
-  Fixpoint up e :=
-    match e with
-    | EAtom op => TAtom op op
+    | EAtom op => op
     | EBinOp lhs rhs =>
-        let uLhs := up lhs in
-        let uRhs := up rhs in
-        let s := max (size uLhs) (size uRhs) in
-        TBinOp s uLhs uRhs
+        let lhs_size := determine lhs in
+        let rhs_size := determine rhs in
+        max lhs_size rhs_size
     | EUnOp arg =>
-        let uArg := up arg in
-        TUnOp (size uArg) uArg
-    | ECast arg =>
-        let uArg := up arg in
-        TCast (size uArg) uArg
-    | EComp lhs rhs =>
-        let uLhs := up lhs in
-        let uRhs := up rhs in
-        TComp 1 uLhs uRhs
-    | ELogic lhs rhs =>
-        let uLhs := up lhs in
-        let uRhs := up rhs in
-        TLogic 1 uLhs uRhs
-    | EReduction arg =>
-        let uArg := up arg in
-        TReduction 1 uArg
+        let arg_size := determine arg in
+        arg_size
+    | EComp lhs rhs => 1
+    | ELogic lhs rhs => 1
+    | EReduction arg => 1
     | EShift lhs rhs =>
-        let uLhs := up lhs in
-        let uRhs := up rhs in
-        TShift (size uLhs) uLhs uRhs
-    | EAssign lval arg =>
-        let uArg := up arg in
-        TAssign lval lval uArg
+        let lhs_size := determine lhs in
+        lhs_size
+    | EAssign lval_size arg => lval_size
     | ECond arg lhs rhs =>
-        let uArg := up arg in
-        let uLhs := up lhs in
-        let uRhs := up rhs in
-        let s := max (size uLhs) (size uRhs) in
-        TCond s uArg uLhs uRhs
+        let lhs_size := determine lhs in
+        let rhs_size := determine rhs in
+        max lhs_size rhs_size
     | EConcat args =>
-        let uArgs := map up args in
-        let s := sum (map size uArgs) in
-        TConcat s uArgs
+        let exprs_size := map determine args in
+        sum exprs_size
     | ERepl n arg =>
-        let uArg := up arg in
-        TReduction (n * (size uArg)) uArg
+        let arg_size := determine arg in
+        n * arg_size
     end
   .
 
-  Definition type e := let tE := up e in down (size tE) tE.
+  Fixpoint propagate e target_size :=
+    let annotate := TExpr in
+    match e with
+    | EAtom op => annotate (TAtom op) target_size
+    | EBinOp lhs rhs =>
+        let ann_lhs := propagate lhs target_size in
+        let ann_rhs := propagate rhs target_size in
+        annotate (TBinOp ann_lhs ann_rhs) target_size
+    | EUnOp arg =>
+        let ann_arg := propagate arg target_size in
+        annotate (TUnOp ann_arg) target_size
+    | EComp lhs rhs =>
+        let lhs_size := determine lhs in
+        let rhs_size := determine rhs in
+        let arg_size := max lhs_size rhs_size in
+        let ann_lhs := propagate lhs arg_size in
+        let ann_rhs := propagate rhs arg_size in
+        annotate (TComp ann_lhs ann_rhs) target_size
+    | ELogic lhs rhs =>
+        let lhs_size := determine lhs in
+        let ann_lhs := propagate lhs lhs_size in
+        let rhs_size := determine rhs in
+        let ann_rhs := propagate rhs rhs_size in
+        annotate (TLogic ann_lhs ann_rhs) target_size
+    | EReduction arg =>
+        let arg_size := determine arg in
+        let ann_arg := propagate arg arg_size in
+        annotate (TReduction ann_arg) target_size
+    | EShift lhs rhs =>
+        let ann_lhs := propagate lhs target_size in
+        let rhs_size := determine rhs in
+        let ann_rhs := propagate rhs rhs_size in
+        annotate (TShift ann_lhs ann_rhs) target_size
+    | EAssign lval_size rhs =>
+        let rhs_size := determine rhs in
+        let arg_size := max lval_size rhs_size in
+        let ann_rhs := propagate rhs arg_size in
+        annotate (TAssign lval_size ann_rhs) target_size
+    | ECond cond true_expr false_expr =>
+        let cond_size := determine cond in
+        let ann_cond := propagate cond cond_size in
+        let ann_true := propagate true_expr target_size in
+        let ann_false := propagate false_expr target_size in
+        annotate (TCond ann_cond ann_true ann_false) target_size
+    | EConcat args =>
+        let ann_args := map (fun expr_i => let expr_i_size := determine expr_i in
+                                        propagate expr_i expr_i_size) args in
+        annotate (TConcat ann_args) target_size
+    | ERepl n inner_expr =>
+        let inner_size := determine inner_expr in
+        let ann_inner := propagate inner_expr inner_size in
+        annotate (TRepl n ann_inner) target_size
+    end
+  .
 
-  Definition size_at e p := option_map size (e @@[p]).
+  Definition type e :=
+    let expr_size := determine e in
+    propagate e expr_size.
 
-  Lemma down_shape1 : forall e p, IsTypedPath e p -> forall s, IsTypedPath (down s e) p.
+  Definition size_at {T: Type} (e: TaggedExpr T) p := option_map tag (e @@[p]).
+
+  Lemma down_shape1 : forall e p,
+      IsPath e p -> forall s, IsTypedPath (propagate e s) p.
   Proof.
     intros. generalize dependent s. induction H; intros; simpl in *;
       econstructor; firstorder.
       rewrite nth_error_map. rewrite H. reflexivity.
   Qed.
 
-  Lemma down_shape2 : forall e p s, IsTypedPath (down s e) p -> IsTypedPath e p.
+  Lemma down_shape2 : forall e p s, IsTypedPath (propagate e s) p -> IsPath e p.
   Proof.
     induction e; intros; try (inv H; constructor; firstorder).
     inv H0. constructor. destruct (nth_error args n) eqn:Hnth;
@@ -114,75 +131,29 @@ Module Algo.
     econstructor. eassumption. apply (H _ _ Hnth _ _ H5).
   Qed.
 
-  Theorem down_shape : forall e p, IsTypedPath e p <-> forall s, IsTypedPath (down s e) p.
+  Theorem down_shape : forall e p, IsPath e p <-> forall s, IsTypedPath (propagate e s) p.
   Proof.
     split; intros.
     - apply (down_shape1 _ _ H).
     - apply (down_shape2 _ _ 0 (H _)).
   Qed.
 
-  Theorem up_shape : forall e p, IsPath e p <-> IsTypedPath (up e) p.
-  Proof.
-    split; intros.
-    - induction H; simpl in *; simpl in *; try (constructor; assumption).
-      econstructor.
-      + rewrite nth_error_map. rewrite H. reflexivity.
-      + assumption.
-    - generalize dependent p. induction e; intros; simpl in *;
-        try (inv H; constructor; firstorder).
-      inv H0. constructor. destruct (nth_error args n) eqn:Hnth;
-        rewrite nth_error_map in *; rewrite Hnth in *; inv H3. econstructor.
-      + eassumption.
-      + firstorder.
-  Qed.
-
   Theorem type_shape : forall e p, IsPath e p <-> IsTypedPath (type e) p.
   Proof.
     split; intros; unfold type in *.
-    - rewrite up_shape in H. apply (down_shape1 _ _ H _).
-    - apply up_shape. apply (down_shape2 _ _ _ H).
+    - apply (down_shape1 _ _ H _).
+    - apply (down_shape2 _ _ _ H).
   Qed.
 
-  Lemma up_top_size : forall e, size (up e) = determine e.
-  Proof.
-    induction e using Expr_ind; simpl; firstorder.
-    induction args.
-    - reflexivity.
-    - simpl. rewrite (H 0). rewrite IHargs. reflexivity. intros n.
-      apply (H (S n)). reflexivity.
-  Qed.
+  Lemma up_top_size : forall e, determine e = Spec.determine e.
+  Proof. induction e using Expr_ind; reflexivity. Qed.
 
-  Lemma down_top_size : forall e s, size (down s e) = s.
-  Proof.
-    intros; destruct e; reflexivity.
-  Qed.
+  Lemma down_top_size : forall e s, tag (propagate e s) = s.
+  Proof. intros; destruct e; reflexivity. Qed.
 
-  Lemma type_top_size : forall e, size (type e) = determine e.
+  Lemma type_top_size : forall e, tag (type e) = determine e.
   Proof.
     intros. unfold type. rewrite up_top_size. apply down_top_size.
-  Qed.
-
-  Theorem up_size_path : forall e p, size_at (up e) p = option_map determine (e @[p]).
-  Proof.
-    intros; unfold size_at; destruct (IsPath_dec e p).
-    - assert (HpTe: IsTypedPath (up e) p) by (apply up_shape; assumption).
-      induction i; try (inv HpTe; firstorder).
-      + rewrite sub_expr_nil. rewrite sub_typed_expr_nil. simpl.
-        rewrite up_top_size. reflexivity.
-      + simpl. rewrite H3. rewrite nth_error_map in H3. rewrite H in *. inv H3.
-        firstorder.
-    - assert (Hse: e @[p] = None). {
-          destruct (e @[p]) eqn:Hse.
-          - exfalso. apply n. apply (sub_expr_valid _ _ _ Hse).
-          - reflexivity.
-      }
-      assert (HsTe: up e @@[p] = None). {
-        destruct (up e @@[p]) eqn:HsTe.
-        - exfalso. apply n. apply sub_typed_expr_valid in HsTe.
-          rewrite <- up_shape in HsTe. assumption.
-        - reflexivity.
-      }
-      rewrite Hse. rewrite HsTe. reflexivity.
   Qed.
 
   Ltac inv_path :=
@@ -192,11 +163,11 @@ Module Algo.
   .
 
   Lemma down_size_path_lemma :
-    forall e s fc, e <== s -| fc -> forall p, IsPath e p -> fc p = size_at (down s (up e)) p.
+    forall e s fc, e <== s -| fc -> forall p, IsPath e p -> fc p = size_at (propagate e s) p.
   Proof.
     Ltac _down_size_dec :=
       match goal with
-      | [ |- _ = option_map _ (down (max ?n ?m) _ @@[_]) ] =>
+      | [ |- _ = option_map _ ((propagate _ (max ?n ?m)) @@[_]) ] =>
           let nH := fresh in destruct (max_dec_bis n m) as [[nH ?]|[nH ?]];
                              rewrite nH in *; clear nH
       end
@@ -207,7 +178,7 @@ Module Algo.
       | [ H: _ -> _ |- _ ] => eapply H; eassumption
       | [ H: _ ==> _ -| _ |- _ ] =>
           learn (synth_must_be_determine _ _ _ H); splitHyp; subst
-      | [ H: ?e ==> determine ?e -| _ |- _ ] =>
+      | [ H: ?e ==> Spec.determine ?e -| _ |- _ ] =>
           learn (synth_can_check _ _ _ _ H (le_refl _)); existsHyp
       | [ H: ?e ==> ?t -| ?f1, F: ?e <== ?t -| ?f2 |- _ ] =>
           let nH := fresh in assert (nH: f1 = f2) by
@@ -216,36 +187,37 @@ Module Algo.
       | [ H: ?e1 ==> ?t -| _, F: ?e2 <== ?t -| _ |- _ ] =>
           learn (synth_check_determine_order _ _ _ _ _ _ H F (le_refl _));
           try antisym; subst
-      | [ H: ?e <== ?t -| _, F: ?t <= determine ?e |- _ ] =>
+      | [ H: ?e <== ?t -| _, F: ?t <= Spec.determine ?e |- _ ] =>
           learn (synth_and_order _ _ _ H F); subst
+      | [ H : context [Spec.determine _] |- _ ] => rewrite up_top_size in H
       end
     .
     induction e using Expr_ind; intros; simpl in *; unfold size_at; inv_path;
       try (apply check_root in H; simpl; congruence);
-      inv_ts; simpl; repeat (rewrite up_top_size);
-      try _down_size_dec; repeat _down_size_p_lem; try lia; try reflexivity.
+      inv_ts; simpl; repeat (rewrite up_top_size); try _down_size_dec;
+      repeat _down_size_p_lem; try lia; try reflexivity.
     repeat (gen_nth). repeat (rewrite nth_error_map). rewrite H3. rewrite H0. simpl.
     repeat (rewrite up_top_size). specialize (H8 _ _ _ _ H3 H1 H0).
     repeat _down_size_p_lem.
   Qed.
 
   Theorem down_size_path : forall e s,
-      determine e <= s -> e <== s -| size_at (down s (up e)).
+      determine e <= s -> e <== s -| size_at (propagate e s).
   Proof.
     intros. destruct (always_synth e) as [t [f Hs]].
     destruct (synth_must_be_determine _ _ _ Hs). subst. clear H1.
     destruct (synth_can_check _ _ _ _ Hs H) as [fc Hc]. clear Hs. clear f.
-    assert (Hfc: fc = size_at (down s (up e))).
+    assert (Hfc: fc = size_at (propagate e s)).
     {
       extensionality p.
       destruct (fc p) eqn:Hfc.
       - assert (Hp: IsPath e p) by (rewrite (check_f_path _ _ _ Hc); exists n; assumption).
         rewrite <- Hfc. apply down_size_path_lemma; assumption.
-      - assert (Hp: ~(IsTypedPath (down s (up e)) p)).
-        { unfold not. intros. apply down_shape2 in H0. rewrite <- up_shape in H0.
+      - assert (Hp: ~(IsTypedPath (propagate e s) p)).
+        { unfold not. intros. apply down_shape2 in H0.
           rewrite (check_f_path _ _ _ Hc) in H0. destruct H0. congruence. }
-        unfold size_at. destruct (down s (up e) @@[ p]) eqn:HsTe.
-        + exfalso. apply Hp. apply (sub_typed_expr_valid _ _ _ HsTe).
+        unfold size_at. destruct (propagate e s @@[ p]) eqn:HsTe.
+        + exfalso. apply Hp. apply (sub_typed_expr_valid _ _ _ _ HsTe).
         + reflexivity.
     }
     rewrite <- Hfc. assumption.
