Rocq/src/TaggedExpr.v
@@ -1,0 +1,132 @@
+From Stdlib Require Import Lists.List.
+
+From Verilog Require Import Utils.
+
+Import ListNotations.
+
+Import Utils.
+
+Module TaggedExpr.
+  Section TaggedExpr_def.
+    Variable T: Type.
+
+    Unset Elimination Schemes.
+
+    Inductive TaggedExprKind : Type :=
+    | TAtom (origSize: nat)
+    | TBinOp (lhs rhs: TaggedExpr)
+    | TUnOp (arg: TaggedExpr)
+    | TComp (lhs rhs: TaggedExpr)
+    | TLogic (lhs rhs: TaggedExpr)
+    | TReduction (arg: TaggedExpr)
+    | TShift (lhs rhs: TaggedExpr)
+    | TAssign (lval: nat) (arg: TaggedExpr)
+    | TCond (cond tb fb: TaggedExpr)
+    | TConcat (args: list TaggedExpr)
+    | TRepl (amount: nat) (arg: TaggedExpr)
+    with TaggedExpr : Type :=
+    | TExpr (body: TaggedExprKind) (tag: T)
+    .
+
+    Set Elimination Schemes.
+
+    Variable P : TaggedExpr -> Prop.
+
+    Hypothesis HPTAtom:
+      forall tag o, P (TExpr (TAtom o) tag).
+
+    Hypothesis HPTBinOp:
+      forall tag lhs rhs, P lhs -> P rhs -> P (TExpr (TBinOp lhs rhs) tag).
+
+    Hypothesis HPTUnOp:
+      forall tag arg, P arg -> P (TExpr (TUnOp arg) tag).
+
+    Hypothesis HPTComp:
+      forall tag lhs rhs, P lhs -> P rhs -> P (TExpr (TComp lhs rhs) tag).
+
+    Hypothesis HPTLogic:
+      forall tag lhs rhs, P lhs -> P rhs -> P (TExpr (TLogic lhs rhs) tag).
+
+    Hypothesis HPTReduction:
+      forall tag arg, P arg -> P (TExpr (TReduction arg) tag).
+
+    Hypothesis HPTShift:
+      forall tag lhs rhs, P lhs -> P rhs -> P (TExpr (TShift lhs rhs) tag).
+
+    Hypothesis HPTAssign:
+      forall tag op arg, P arg -> P (TExpr (TAssign op arg) tag).
+
+    Hypothesis HPTCond:
+      forall tag cond tb fb, P cond -> P tb -> P fb -> P (TExpr (TCond cond tb fb) tag).
+
+    Hypothesis HPTConcat:
+      forall tag args, (forall n e, nth_error args n = Some e -> P e) -> P (TExpr (TConcat args) tag).
+
+    Hypothesis HPTRepl:
+      forall tag n arg, P arg -> P (TExpr (TRepl n arg) tag).
+
+    Lemma HNil: forall n e, nth_error [] n = Some e -> P e.
+    Proof. intros; destruct n; inv H. Qed.
+
+    Lemma HCons: forall hd tl,
+        P hd -> (forall n e, nth_error tl n = Some e -> P e) ->
+        forall n e, nth_error (hd :: tl) n = Some e -> P e.
+    Proof.
+      intros; destruct n; inv H1.
+      - apply H.
+      - apply (H0 _ _ H3).
+    Qed.
+
+    Fixpoint TaggedExpr_ind e : P e :=
+      match e with
+      | TExpr eKind tag =>
+          match eKind with
+          | TAtom o =>
+              HPTAtom tag o
+          | TBinOp lhs rhs =>
+              HPTBinOp tag _ _ (TaggedExpr_ind lhs) (TaggedExpr_ind rhs)
+          | TUnOp arg =>
+              HPTUnOp tag _ (TaggedExpr_ind arg)
+          | TComp lhs rhs =>
+              HPTComp tag _ _ (TaggedExpr_ind lhs) (TaggedExpr_ind rhs)
+          | TLogic lhs rhs =>
+              HPTLogic tag _ _ (TaggedExpr_ind lhs) (TaggedExpr_ind rhs)
+          | TReduction arg =>
+              HPTReduction tag _ (TaggedExpr_ind arg)
+          | TShift lhs rhs =>
+              HPTShift tag _ _ (TaggedExpr_ind lhs) (TaggedExpr_ind rhs)
+          | TAssign lval arg =>
+              HPTAssign tag lval _ (TaggedExpr_ind arg)
+          | TCond arg lhs rhs =>
+              HPTCond tag _ _ _ (TaggedExpr_ind arg) (TaggedExpr_ind lhs) (TaggedExpr_ind rhs)
+          | TConcat args =>
+              HPTConcat tag args
+                ((list_ind _ HNil
+                    (fun hd tl => HCons _ tl (TaggedExpr_ind hd))) args)
+          | TRepl n arg =>
+              HPTRepl tag n _ (TaggedExpr_ind arg)
+          end
+      end
+    .
+
+  End TaggedExpr_def.
+
+  Arguments TAtom {T}.
+  Arguments TBinOp {T}.
+  Arguments TUnOp {T}.
+  Arguments TComp {T}.
+  Arguments TLogic {T}.
+  Arguments TReduction {T}.
+  Arguments TShift {T}.
+  Arguments TAssign {T}.
+  Arguments TCond {T}.
+  Arguments TConcat {T}.
+  Arguments TRepl {T}.
+  Arguments TExpr {T}.
+
+  Definition tag {T: Type} (e: TaggedExpr T) :=
+    match e with
+    | TExpr _ tag => tag
+    end
+  .
+End TaggedExpr.
