Rocq/src/TaggedExprPath.v
@@ -1,0 +1,166 @@
+From Stdlib Require Import Lists.List.
+
+From Verilog Require Import TaggedExpr.
+From Verilog Require Export Path.
+From Verilog Require Import Utils.
+
+Import ListNotations.
+
+Import TaggedExpr.
+Import Path.
+Import Utils.
+
+Module TaggedExprPath.
+  Inductive IsTypedPath {T: Type} : TaggedExpr T -> path -> Prop :=
+  | TP_Empty : forall e,
+      IsTypedPath e []
+  | TP_LhsBinOp : forall tag lhs rhs p,
+      IsTypedPath lhs p ->
+      IsTypedPath (TExpr (TBinOp lhs rhs) tag) (0 :: p)
+  | TP_RhsBinOp : forall tag lhs rhs p,
+      IsTypedPath rhs p ->
+      IsTypedPath (TExpr (TBinOp lhs rhs) tag) (1 :: p)
+  | TP_UnOpArg : forall tag arg p,
+      IsTypedPath arg p ->
+      IsTypedPath (TExpr (TUnOp arg) tag) (0 :: p)
+  | TP_LhsCompOp : forall tag lhs rhs p,
+      IsTypedPath lhs p ->
+      IsTypedPath (TExpr (TComp lhs rhs) tag) (0 :: p)
+  | TP_RhsCompOp : forall tag lhs rhs p,
+      IsTypedPath rhs p ->
+      IsTypedPath (TExpr (TComp lhs rhs) tag) (1 :: p)
+  | TP_LhsLogic : forall tag lhs rhs p,
+      IsTypedPath lhs p ->
+      IsTypedPath (TExpr (TLogic lhs rhs) tag) (0 :: p)
+  | TP_RhsLogic : forall tag lhs rhs p,
+      IsTypedPath rhs p ->
+      IsTypedPath (TExpr (TLogic lhs rhs) tag) (1 :: p)
+  | TP_RedArg : forall tag arg p,
+      IsTypedPath arg p ->
+      IsTypedPath (TExpr (TReduction arg) tag) (0 :: p)
+  | TP_LhsShift : forall tag lhs rhs p,
+      IsTypedPath lhs p ->
+      IsTypedPath (TExpr (TShift lhs rhs) tag) (0 :: p)
+  | TP_RhsShift : forall tag lhs rhs p,
+      IsTypedPath rhs p ->
+      IsTypedPath (TExpr (TShift lhs rhs) tag) (1 :: p)
+  | TP_AssignArg : forall tag op arg p,
+      IsTypedPath arg p ->
+      IsTypedPath (TExpr (TAssign op arg) tag) (0 :: p)
+  | TP_CondCond : forall tag cond tb fb p,
+      IsTypedPath cond p ->
+      IsTypedPath (TExpr (TCond cond tb fb) tag) (0 :: p)
+  | TP_CondTrue : forall tag cond tb fb p,
+      IsTypedPath tb p ->
+      IsTypedPath (TExpr (TCond cond tb fb) tag) (1 :: p)
+  | TP_CondFalse : forall tag cond tb fb p,
+      IsTypedPath fb p ->
+      IsTypedPath (TExpr (TCond cond tb fb) tag) (2 :: p)
+  | TP_ConcatArgs : forall tag n args e p,
+      nth_error args n = Some e -> IsTypedPath e p ->
+      IsTypedPath (TExpr (TConcat args) tag) (n :: p)
+  | TP_ReplArg : forall tag i arg p,
+      IsTypedPath arg p ->
+      IsTypedPath (TExpr (TRepl i arg) tag) (0 :: p)
+  .
+
+  Fixpoint sub_typed_expr {T: Type} (e: TaggedExpr T) (p: path) :=
+    match e, p with
+    | e, [] => Some e
+    | TExpr (TBinOp lhs _) _, 0 :: p => sub_typed_expr lhs p
+    | TExpr (TBinOp _ rhs) _, 1 :: p => sub_typed_expr rhs p
+    | TExpr (TUnOp arg) _, 0 :: p => sub_typed_expr arg p
+    | TExpr (TComp lhs _) _, 0 :: p => sub_typed_expr lhs p
+    | TExpr (TComp _ rhs) _, 1 :: p => sub_typed_expr rhs p
+    | TExpr (TLogic lhs _) _, 0 :: p => sub_typed_expr lhs p
+    | TExpr (TLogic _ rhs) _, 1 :: p => sub_typed_expr rhs p
+    | TExpr (TReduction arg) _, 0 :: p => sub_typed_expr arg p
+    | TExpr (TShift lhs _) _, 0 :: p => sub_typed_expr lhs p
+    | TExpr (TShift _ rhs) _, 1 :: p => sub_typed_expr rhs p
+    | TExpr (TAssign _ arg) _, 0 :: p => sub_typed_expr arg p
+    | TExpr (TCond cond _ _) _, 0 :: p => sub_typed_expr cond p
+    | TExpr (TCond _ tb _) _, 1 :: p => sub_typed_expr tb p
+    | TExpr (TCond _ _ fb) _, 2 :: p => sub_typed_expr fb p
+    | TExpr (TConcat args) _, i :: p =>
+        match nth_error args i with
+        | Some e => sub_typed_expr e p
+        | None => None
+        end
+    | TExpr (TRepl _ arg) _, 0 :: p => sub_typed_expr arg p
+    | TExpr _ _, _ :: _ => None
+    end
+  .
+
+  Notation "e @@[ p ]" := (sub_typed_expr e p) (at level 20).
+
+  Lemma sub_typed_expr_nil: forall T (e: TaggedExpr T), e @@[[]] = Some e.
+  Proof.
+    intros. destruct e as [[]]; reflexivity.
+  Qed.
+
+  Lemma IsTypedPath_is_sub_typed_expr: forall T (e: TaggedExpr T) p,
+      IsTypedPath e p -> exists e0, e @@[p] = Some e0.
+  Proof.
+    intros. induction H; try (destruct IHIsTypedPath as [x H1]; exists x; assumption).
+    - exists e. apply sub_typed_expr_nil.
+    - destruct IHIsTypedPath as [x H1]; exists x. simpl. rewrite H. assumption.
+  Qed.
+
+  Lemma sub_typed_expr_valid: forall T (e: TaggedExpr T) p f,
+      e @@[p] = Some f -> IsTypedPath e p.
+  Proof.
+    induction e using TaggedExpr_ind; intros;
+      try (destruct p as [|[|[|[]]]]; simpl in *;
+           (constructor; firstorder) || congruence).
+    - destruct p.
+      + constructor.
+      + destruct (nth_error args n) eqn:H1; simpl in H0; rewrite H1 in H0.
+        * apply (TP_ConcatArgs _ _ _ _ _ H1 (H _ _ H1 _ _ H0)).
+        * congruence.
+  Qed.
+
+  Lemma IsTypedPath_sub_typed_expr_iff:
+    forall T (e: TaggedExpr T) p, IsTypedPath e p <-> exists e0, e @@[p] = Some e0.
+  Proof.
+    split.
+    - apply IsTypedPath_is_sub_typed_expr.
+    - intros [? H]. apply (sub_typed_expr_valid _ _ _ _ H).
+  Qed.
+
+  Lemma sub_typed_expr_chunk : forall T p q (e: TaggedExpr T) g,
+      (exists f, e @@[p] = Some f /\ f @@[q] = Some g) <-> e @@[p ++ q] = Some g.
+  Proof.
+    induction p; split; intros.
+    - destruct H as [f [H1 H2]]. rewrite sub_typed_expr_nil in H1. inv H1. assumption.
+    - exists e. split. apply sub_typed_expr_nil. assumption.
+    - destruct H as [f [H1 H2]]. destruct e as [[]]; simpl in *;
+        try congruence; try (destruct (nth_error _ a)); destruct a as [|[|[]]];
+        congruence || (apply IHp; eexists; intuition; eassumption).
+    - destruct e as [[]]; simpl in *;
+        try congruence; try (destruct (nth_error _ a));
+        destruct a as [|[|[]]]; congruence || apply IHp; assumption.
+  Qed.
+
+  Lemma IsTypedPath_chunk : forall T (e: TaggedExpr T) p c,
+      IsTypedPath e (p ++ c) <-> (exists f, e @@[p] = Some f /\ IsTypedPath f c).
+  Proof.
+    split; intros.
+    - destruct (IsTypedPath_is_sub_typed_expr _ _ _ H) as [g H1].
+      apply sub_typed_expr_chunk in H1.
+      destruct H1 as [f [H2 H3]]. exists f. split. assumption.
+      apply IsTypedPath_sub_typed_expr_iff.
+      exists g. assumption.
+    - destruct H as [f [H1 H2]]. apply IsTypedPath_sub_typed_expr_iff.
+      apply IsTypedPath_sub_typed_expr_iff in H2. destruct H2 as [g H2]. exists g.
+      apply sub_typed_expr_chunk. exists f. intuition.
+  Qed.
+
+  Theorem IsTypedPath_dec : forall T (e: TaggedExpr T) p,
+      {IsTypedPath e p} + {~(IsTypedPath e p)}.
+  Proof.
+    intros. destruct (e @@[p]) eqn:Hep.
+    - left. apply (sub_typed_expr_valid _ _ _ _ Hep).
+    - right. unfold not. intros. rewrite IsTypedPath_sub_typed_expr_iff in H. destruct H.
+      congruence.
+  Qed.
+End TaggedExprPath.
